Tightening up assembly code

12AssemblyCode/Assemble.thy
@@ -14,13 +14,13 @@ primrec assemble_op :: "(nat \<Rightarrow> nat) \<Rightarrow> code\<^sub>b \<Rig
   "assemble_op mp (Lookup\<^sub>b x) = [
     AMov (Con 0),
     AAdd (Reg Vals) 1,
-    APut Vals (Acc (Con 0)),
-    AGet (Acc (Reg Env)) (Reg Hp),
+    APut Vals (Acc (Reg Hp)),
+    AGet (Acc (Reg Env)),
     ASub (Acc (Reg Env)) 2] @
     concat (replicate x [
-    AGet (Acc (Reg Env)) (Reg Env),
+    AGet (Acc (Reg Env)),
     ASub (Acc (Reg Env)) 1]) @ [
-    AGet (Acc (Reg Stk)) (Reg Env),
+    AGet (Acc (Reg Stk)),
     ASub (Acc (Reg Stk)) 1,
     AMov (Reg Stk)]"
 | "assemble_op mp (PushCon\<^sub>b k) = [
@@ -37,67 +37,67 @@ primrec assemble_op :: "(nat \<Rightarrow> nat) \<Rightarrow> code\<^sub>b \<Rig
     APut Hp (PC (mp pc)), 
     AMov (Con 0),
     AAdd (Reg Hp) 1, 
-    APut Hp (Acc (Con 0)),
+    APut Hp (Acc (Reg Env)),
     AAdd (Reg Hp) 1, 
     APut Hp (Con 0),
-    AGet (Acc (Reg Stk)) (Reg Env), 
+    AGet (Acc (Reg Stk)), 
     ASub (Acc (Reg Stk)) 1,
     AMov (Reg Stk),
     AAdd (Reg Vals) 1,
     APut Vals (Reg Hp)]"
 | "assemble_op mp Apply\<^sub>b = [
     AJmp,
-    AGet (Acc (Reg Hp)) (PC 0),
+    AGet (Acc (Reg Hp)),
     AAdd (Acc (Reg Hp)) 2,
     APut Vals (Con 0),
-    AGet (Reg Vals) (Reg Hp),
+    AGet (Reg Vals),
     AAdd (Reg Env) 1,
-    APut Env (Acc (Con 0)),
-    AGet (Acc (Reg Hp)) (Reg Env),
+    APut Env (Acc (Reg Env)),
+    AGet (Acc (Reg Hp)),
     AAdd (Acc (Reg Hp)) 1,
-    AGet (Reg Vals) (Reg Hp),
+    AGet (Reg Vals),
     ASub (Reg Vals) 1,
     AAdd (Reg Stk) 1,
-    APut Stk (Acc (Con 0)),
+    APut Stk (Acc (Reg Env)),
     AAdd (Acc (Reg Env)) 1,
     AMov (Reg Env),
     AAdd (Reg Stk) 1,
-    APut Stk (Acc (Con 0)),
+    APut Stk (Acc (PC 0)),
     ASub (Acc (PC 0)) 18,
     AMov (PC 0),
     AAdd (Reg Env) 1,
-    APut Env (Acc (Con 0)),
+    APut Env (Acc (Reg Hp)),
     APut Vals (Con 0),
-    AGet (Reg Vals) (Reg Hp),
+    AGet (Reg Vals),
     ASub (Reg Vals) 1]"
 | "assemble_op mp Return\<^sub>b = [
     AJmp,
     APut Stk (Con 0),
-    AGet (Reg Stk) (PC 0),
+    AGet (Reg Stk),
     ASub (Reg Stk) 1,
     APut Stk (Con 0),
     ASub (Reg Stk) 1]"
 | "assemble_op mp Jump\<^sub>b = [
     AJmp,
-    AGet (Acc (Reg Hp)) (PC 0),
+    AGet (Acc (Reg Hp)),
     AAdd (Acc (Reg Hp)) 2,
     APut Vals (Con 0),
-    AGet (Reg Vals) (Reg Hp),
+    AGet (Reg Vals),
     AAdd (Reg Env) 1,
-    APut Env (Acc (Con 0)),
-    AGet (Acc (Reg Hp)) (Reg Env),
+    APut Env (Acc (Reg Env)),
+    AGet (Acc (Reg Hp)),
     AAdd (Acc (Reg Hp)) 1,
-    AGet (Reg Vals) (Reg Hp),
+    AGet (Reg Vals),
     ASub (Reg Vals) 1,
     AAdd (Reg Stk) 1,
-    APut Stk (Acc (Con 0)),
+    APut Stk (Acc (Reg Env)),
     ASub (Reg Stk) 1,
     AAdd (Acc (Reg Env)) 1,
     AMov (Reg Env),
     AAdd (Reg Env) 1,
-    APut Env (Acc (Con 0)),
+    APut Env (Acc (Reg Hp)),
     APut Vals (Con 0),
-    AGet (Reg Vals) (Reg Hp),
+    AGet (Reg Vals),
     ASub (Reg Vals) 1]"
 
 fun assembly_map :: "code\<^sub>b list \<Rightarrow> nat \<Rightarrow> nat" where
@@ -109,32 +109,32 @@ definition assemble_code :: "code\<^sub>b list \<Rightarrow> assm list" where
   "assemble_code cd = concat (map (assemble_op (assembly_map cd)) cd)"
 
 definition assemble_heap :: "(nat \<Rightarrow> nat) \<Rightarrow> (nat \<Rightarrow> pointer_tag \<times> nat) \<Rightarrow> nat \<Rightarrow> nat \<Rightarrow> 
-    pseudoreg \<times> nat" where
-  "assemble_heap mp h hp x = (if x \<ge> hp then (Con 0, 0) else case x mod 3 of
-      0 \<Rightarrow> (Con 0, snd (h x))
-    | Suc 0 \<Rightarrow> (if snd (h (x - 1)) = 0 then Reg Env else Con 0, snd (h x))
-    | Suc (Suc 0) \<Rightarrow> if snd (h (x - 2)) = 0 then (PC 0, mp (snd (h x))) else (Con 0, snd (h x)))"
+    register option \<times> nat" where
+  "assemble_heap mp h hp x = (if x \<ge> hp then (None, 0) else case x mod 3 of
+      0 \<Rightarrow> (None, snd (h x))
+    | Suc 0 \<Rightarrow> (if snd (h (x - 1)) = 0 then Some Env else None, snd (h x))
+    | Suc (Suc 0) \<Rightarrow> if snd (h (x - 2)) = 0 then (None, mp (snd (h x))) else (None, snd (h x)))"
 
-definition assemble_env :: "(nat \<Rightarrow> nat) \<Rightarrow> nat \<Rightarrow> nat \<Rightarrow> pseudoreg \<times> nat" where
-  "assemble_env e ep x = (if x \<ge> ep then (Con 0, 0) else (Reg (if even x then Hp else Env), e x))"
+definition assemble_env :: "(nat \<Rightarrow> nat) \<Rightarrow> nat \<Rightarrow> nat \<Rightarrow> register option \<times> nat" where
+  "assemble_env e ep x = (if x \<ge> ep then (None, 0) else (Some (if even x then Hp else Env), e x))"
 
-definition assemble_vals :: "(nat \<Rightarrow> nat) \<Rightarrow> nat \<Rightarrow> nat \<Rightarrow> pseudoreg \<times> nat" where
-  "assemble_vals vs vp x = (if x \<ge> vp then (Con 0, 0) else (Reg Hp, vs x))"
+definition assemble_vals :: "(nat \<Rightarrow> nat) \<Rightarrow> nat \<Rightarrow> nat \<Rightarrow> register option \<times> nat" where
+  "assemble_vals vs vp x = (if x \<ge> vp then (None, 0) else (Some Hp, vs x))"
 
-definition assemble_stack :: "(nat \<Rightarrow> nat) \<Rightarrow> (nat \<Rightarrow> nat) \<Rightarrow> nat \<Rightarrow> nat \<Rightarrow> pseudoreg \<times> nat" where
+definition assemble_stack :: "(nat \<Rightarrow> nat) \<Rightarrow> (nat \<Rightarrow> nat) \<Rightarrow> nat \<Rightarrow> nat \<Rightarrow> register option \<times> nat" where
   "assemble_stack mp s sp x = (
-    if x \<ge> sp then (Con 0, 0) else if even x then (PC 0, mp (s x)) else (Reg Env, s x))"
+    if x \<ge> sp then (None, 0) else if even x then (None, mp (s x)) else (Some Env, s x))"
 
 primrec assemble_state :: "(nat \<Rightarrow> nat) \<Rightarrow> unstr_state \<Rightarrow> assm_state" where
   "assemble_state mp (S\<^sub>u h hp e ep vs vp sh sp pc) = 
     AS (case_register (assemble_heap mp h hp) (assemble_env e ep) (assemble_vals vs vp) 
-      (assemble_stack mp sh sp)) (case_register hp ep vp sp) 0 (Con 0) (mp pc)"
+      (assemble_stack mp sh sp)) (case_register hp ep vp sp) 0 None (mp pc)"
 
-abbreviation assm_hp :: "code\<^sub>b list \<Rightarrow> (nat \<Rightarrow> pointer_tag \<times> nat) \<Rightarrow> nat \<Rightarrow> nat \<Rightarrow> pseudoreg \<times> nat" 
-    where
+abbreviation assm_hp :: "code\<^sub>b list \<Rightarrow> (nat \<Rightarrow> pointer_tag \<times> nat) \<Rightarrow> nat \<Rightarrow> nat \<Rightarrow> 
+    register option \<times> nat" where
   "assm_hp cd \<equiv> assemble_heap (assembly_map cd)"
 
-abbreviation assm_stk :: "code\<^sub>b list \<Rightarrow> (nat \<Rightarrow> nat) \<Rightarrow> nat \<Rightarrow> nat \<Rightarrow> pseudoreg \<times> nat" where
+abbreviation assm_stk :: "code\<^sub>b list \<Rightarrow> (nat \<Rightarrow> nat) \<Rightarrow> nat \<Rightarrow> nat \<Rightarrow> register option \<times> nat" where
   "assm_stk cd \<equiv> assemble_stack (assembly_map cd)"
 
 abbreviation assm_state :: "code\<^sub>b list \<Rightarrow> unstr_state \<Rightarrow> assm_state" where
@@ -228,30 +228,30 @@ lemma [simp]: "lookup cd pc = Some op \<Longrightarrow>
     lookup (assemble_code cd) (assembly_map cd pc) = lookup (assemble_op (assembly_map cd) op) 0"
   using assemble_code_lookup by fastforce
 
-lemma assm_hp_lemma1: "3 dvd x \<Longrightarrow> x < hp \<Longrightarrow> assemble_heap mp h hp x = (Con 0, snd (h x))"
+lemma assm_hp_lemma1: "3 dvd x \<Longrightarrow> x < hp \<Longrightarrow> assemble_heap mp h hp x = (None, snd (h x))"
   by (simp add: assemble_heap_def)
 
 lemma assm_hp_lemma2: "x mod 3 = 1 \<Longrightarrow> snd (h (x - 1)) \<noteq> 0 \<Longrightarrow> x < hp \<Longrightarrow> 
-    assemble_heap mp h hp x = (Con 0, snd (h x))"
+    assemble_heap mp h hp x = (None, snd (h x))"
   by (simp add: assemble_heap_def)
 
 lemma assm_hp_lemma3: "x mod 3 = 1 \<Longrightarrow> snd (h (x - 1)) = 0 \<Longrightarrow> x < hp \<Longrightarrow>
-    assemble_heap mp h hp x = (Reg Env, snd (h x))"
+    assemble_heap mp h hp x = (Some Env, snd (h x))"
   by (simp add: assemble_heap_def)
 
 lemma assm_hp_lemma4: "x mod 3 = 2 \<Longrightarrow> snd (h (x - 2)) \<noteq> 0 \<Longrightarrow> x < hp \<Longrightarrow> 
-    assemble_heap mp h hp x = (Con 0, snd (h x))"
+    assemble_heap mp h hp x = (None, snd (h x))"
   by (simp add: assemble_heap_def)
 
 lemma assm_hp_lemma5: "x mod 3 = 2 \<Longrightarrow> snd (h (x - 2)) = 0 \<Longrightarrow> x < hp \<Longrightarrow> 
-    assemble_heap mp h hp x = (PC 0, mp (snd (h x)))"
+    assemble_heap mp h hp x = (None, mp (snd (h x)))"
   by (simp add: assemble_heap_def)
 
 lemma [simp]: "x \<noteq> hp \<Longrightarrow> assm_hp cd (h(hp := a)) (Suc hp) x = assm_hp cd h hp x"
   by (induction x rule: x_mod_3_induct) (simp_all add: assemble_heap_def, linarith+)
 
 lemma [simp]: "restructurable_heap h hp ep (length cd) \<Longrightarrow> (assm_hp cd h hp)
-  (hp := (Con 0, Suc a), Suc hp := (Con 0, b), Suc (Suc hp) := (Con 0, c)) = 
+  (hp := (None, Suc a), Suc hp := (None, b), Suc (Suc hp) := (None, c)) = 
     assm_hp cd (h(hp := (PConst, Suc a), Suc hp := (PConst, b), Suc (Suc hp) := (PConst, c))) 
       (Suc (Suc (Suc hp)))"
 proof
@@ -261,14 +261,14 @@ proof
   moreover hence "Suc hp mod 3 = 1" by presburger
   moreover hence "Suc (Suc hp) mod 3 = 2" by presburger
   ultimately show "((assm_hp cd h hp)
-    (hp := (Con 0, Suc a), Suc hp := (Con 0, b), Suc (Suc hp) := (Con 0, c))) x =
+    (hp := (None, Suc a), Suc hp := (None, b), Suc (Suc hp) := (None, c))) x =
       assm_hp cd (h(hp := (PConst, Suc a), Suc hp := (PConst, b), Suc (Suc hp) := (PConst, c))) 
         (Suc (Suc (Suc hp))) x" 
     by (simp add: assm_hp_lemma1 assm_hp_lemma2 assm_hp_lemma3 assm_hp_lemma4 assm_hp_lemma5)
 qed
 
 lemma [simp]: "restructurable_heap h hp ep (length cd) \<Longrightarrow> (assm_hp cd h hp)
-  (hp := (Con 0, 0), Suc hp := (Reg Env, a), Suc (Suc hp) := (PC 0, assembly_map cd b)) = 
+  (hp := (None, 0), Suc hp := (Some Env, a), Suc (Suc hp) := (None, assembly_map cd b)) = 
     assm_hp cd (h(hp := (PConst, 0), Suc hp := (PEnv, a), Suc (Suc hp) := (PCode, b))) 
       (Suc (Suc (Suc hp)))"
 proof
@@ -277,8 +277,8 @@ proof
   hence H: "3 dvd hp" by (simp add: restructurable_heap_def)
   moreover hence "Suc hp mod 3 = 1" by presburger
   moreover hence "Suc (Suc hp) mod 3 = 2" by presburger
-  ultimately show "((assm_hp cd h hp)(hp := (Con 0, 0), Suc hp := (Reg Env, a), 
-    Suc (Suc hp) := (PC 0, assembly_map cd b))) x =
+  ultimately show "((assm_hp cd h hp)(hp := (None, 0), Suc hp := (Some Env, a), 
+    Suc (Suc hp) := (None, assembly_map cd b))) x =
       assm_hp cd (h(hp := (PConst, 0), Suc hp := (PEnv, a), Suc (Suc hp) := (PCode, b))) 
         (Suc (Suc (Suc hp))) x" 
     by (simp add: assm_hp_lemma1 assm_hp_lemma2 assm_hp_lemma3 assm_hp_lemma4 assm_hp_lemma5)
@@ -286,25 +286,25 @@ qed
 
 lemma [simp]: "restructurable_vals vs (Suc (Suc vp)) hp \<Longrightarrow> 
   assemble_heap mp h hp (Suc (vs vp)) = 
-    (if snd (h (vs vp)) = 0 then Reg Env else Con 0, snd (h (Suc (vs vp))))"
+    (if snd (h (vs vp)) = 0 then Some Env else None, snd (h (Suc (vs vp))))"
 proof (unfold assemble_heap_def restructurable_vals_def)
   assume "3 dvd hp \<and> (\<forall>x<Suc (Suc vp). 3 dvd vs x \<and> vs x < hp)"
   moreover hence X: "3 dvd vs vp \<and> vs vp < hp" by simp
   ultimately have "Suc (vs vp) < hp" by fastforce
   moreover from X have "Suc (vs vp) mod 3 = 1" by presburger
-  ultimately show "(if Suc (vs vp) \<ge> hp then (Con 0, 0) else case Suc (vs vp) mod 3 of 
-       0 \<Rightarrow> (Con 0, snd (h (Suc (vs vp))))
-     | Suc 0 \<Rightarrow> (if snd (h (Suc (vs vp) - 1)) = 0 then Reg Env else Con 0, snd (h (Suc (vs vp))))
-     | Suc (Suc 0) \<Rightarrow> if snd (h (Suc (vs vp) - 2)) = 0 then (PC 0, mp (snd (h (Suc (vs vp))))) 
-        else (Con 0, snd (h (Suc (vs vp))))
-     | Suc (Suc (Suc x)) \<Rightarrow> undefined) = (if snd (h (vs vp)) = 0 then Reg Env 
-        else Con 0, snd (h (Suc (vs vp))))" 
+  ultimately show "(if Suc (vs vp) \<ge> hp then (None, 0) else case Suc (vs vp) mod 3 of 
+       0 \<Rightarrow> (None, snd (h (Suc (vs vp))))
+     | Suc 0 \<Rightarrow> (if snd (h (Suc (vs vp) - 1)) = 0 then Some Env else None, snd (h (Suc (vs vp))))
+     | Suc (Suc 0) \<Rightarrow> if snd (h (Suc (vs vp) - 2)) = 0 then (None, mp (snd (h (Suc (vs vp))))) 
+        else (None, snd (h (Suc (vs vp))))
+     | Suc (Suc (Suc x)) \<Rightarrow> undefined) = (if snd (h (vs vp)) = 0 then Some Env 
+        else None, snd (h (Suc (vs vp))))" 
     by simp
 qed
 
 lemma [simp]: "restructurable_vals vs (Suc (Suc vp)) hp \<Longrightarrow> snd (h (vs vp)) = 0 \<Longrightarrow> 
   restructurable_heap h hp ep lcd \<Longrightarrow>
-    assemble_heap mp h hp (Suc (Suc (vs vp))) = (PC 0, mp (snd (h (Suc (Suc (vs vp))))))"
+    assemble_heap mp h hp (Suc (Suc (vs vp))) = (None, mp (snd (h (Suc (Suc (vs vp))))))"
 proof (unfold assemble_heap_def restructurable_vals_def)
   assume "3 dvd hp \<and> (\<forall>x<Suc (Suc vp). 3 dvd vs x \<and> vs x < hp)"
   hence "3 dvd vs vp \<and> vs vp < hp" by simp
@@ -312,14 +312,14 @@ proof (unfold assemble_heap_def restructurable_vals_def)
   moreover hence "3 dvd hp" by auto
   ultimately have "Suc (Suc (vs vp)) mod 3 = 2 \<and> Suc (Suc (vs vp)) < hp" by presburger
   moreover assume "snd (h (vs vp)) = 0"
-  ultimately show "(if (Suc (Suc (vs vp))) \<ge> hp then (Con 0, 0) else case Suc (Suc (vs vp)) mod 3 of 
-       0 \<Rightarrow> (Con 0, snd (h (Suc (Suc (vs vp)))))
-     | Suc 0 \<Rightarrow> (if snd (h (Suc (Suc (vs vp)) - 1)) = 0 then Reg Env 
-        else Con 0, snd (h (Suc (Suc (vs vp)))))
+  ultimately show "(if (Suc (Suc (vs vp))) \<ge> hp then (None, 0) else case Suc (Suc (vs vp)) mod 3 of 
+       0 \<Rightarrow> (None, snd (h (Suc (Suc (vs vp)))))
+     | Suc 0 \<Rightarrow> (if snd (h (Suc (Suc (vs vp)) - 1)) = 0 then Some Env 
+        else None, snd (h (Suc (Suc (vs vp)))))
      | Suc (Suc 0) \<Rightarrow>
-         if snd (h (Suc (Suc (vs vp)) - 2)) = 0 then (PC 0, mp (snd (h (Suc (Suc (vs vp))))))
-        else (Con 0, snd (h (Suc (Suc (vs vp)))))
-     | Suc (Suc (Suc x)) \<Rightarrow> undefined) = (PC 0, mp (snd (h (Suc (Suc (vs vp))))))" 
+         if snd (h (Suc (Suc (vs vp)) - 2)) = 0 then (None, mp (snd (h (Suc (Suc (vs vp))))))
+        else (None, snd (h (Suc (Suc (vs vp)))))
+     | Suc (Suc (Suc x)) \<Rightarrow> undefined) = (None, mp (snd (h (Suc (Suc (vs vp))))))" 
     by simp
 qed
 
@@ -327,75 +327,75 @@ lemma [simp]: "Suc (Suc (vs vp)) mod 3 \<noteq> Suc (Suc (Suc x))"
   by simp
 
 lemma [simp]: "snd (h (vs vp)) = Suc x \<Longrightarrow> vs vp mod 3 = 0 \<Longrightarrow> Suc (Suc (vs vp)) < hp \<Longrightarrow>
-    assemble_heap mp h hp (Suc (Suc (vs vp))) = (Con 0, snd (h (Suc (Suc (vs vp)))))"
+    assemble_heap mp h hp (Suc (Suc (vs vp))) = (None, snd (h (Suc (Suc (vs vp)))))"
   by (simp add: assemble_heap_def split: nat.splits) presburger
 
 lemma [simp]: "even sp \<Longrightarrow> 
-  (assm_stk cd sh sp)(sp := (PC 0, assembly_map cd pc), Suc sp := (Reg Env, a)) = 
+  (assm_stk cd sh sp)(sp := (None, assembly_map cd pc), Suc sp := (Some Env, a)) = 
     (assm_stk cd (sh(sp := pc, Suc sp := a)) (Suc (Suc sp)))"
   by (auto simp add: assemble_stack_def)
 
 lemma [simp]: "even (Suc sp) \<Longrightarrow> 
-    (assm_stk cd sh (Suc sp))(sp := (Reg Env, k)) = assm_stk cd (sh(sp := k)) (Suc sp)"
+    (assm_stk cd sh (Suc sp))(sp := (Some Env, k)) = assm_stk cd (sh(sp := k)) (Suc sp)"
   by (auto simp add: assemble_stack_def)
 
-lemma [simp]: "even (Suc sp) \<Longrightarrow> assm_stk cd sh (Suc sp) sp = (Reg Env, sh sp)"
+lemma [simp]: "even (Suc sp) \<Longrightarrow> assm_stk cd sh (Suc sp) sp = (Some Env, sh sp)"
   by (simp add: assemble_stack_def)
 
 lemma [simp]: "even (Suc (Suc sp)) \<Longrightarrow> assm_stk cd sh (Suc sp) sp = 
-    (PC 0, assembly_map cd (sh sp))"
+    (None, assembly_map cd (sh sp))"
   by (simp add: assemble_stack_def)
 
-lemma [simp]: "(assm_stk cd sh (Suc sp))(sp := (Con 0, 0)) = assm_stk cd sh sp"
+lemma [simp]: "(assm_stk cd sh (Suc sp))(sp := (None, 0)) = assm_stk cd sh sp"
   by (auto simp add: assemble_stack_def)
 
-lemma [simp]: "(assemble_vals vs vp)(vp := (Reg Hp, y)) = assemble_vals (vs(vp := y)) (Suc vp)"
+lemma [simp]: "(assemble_vals vs vp)(vp := (Some Hp, y)) = assemble_vals (vs(vp := y)) (Suc vp)"
   by (auto simp add: assemble_vals_def)
 
-lemma [simp]: "(assemble_vals vs (Suc vp))(vp := (Con 0, 0)) = assemble_vals vs vp"
+lemma [simp]: "(assemble_vals vs (Suc vp))(vp := (None, 0)) = assemble_vals vs vp"
   by rule (simp add: assemble_vals_def)
 
-lemma [simp]: "even ep \<Longrightarrow> (assemble_env e ep)(ep := (Reg Hp, a), Suc ep := (Reg Env, b)) = 
+lemma [simp]: "even ep \<Longrightarrow> (assemble_env e ep)(ep := (Some Hp, a), Suc ep := (Some Env, b)) = 
     assemble_env (e(ep := a, Suc ep := b)) (Suc (Suc ep))"
   by (auto simp add: assemble_env_def)
 
 lemma [simp]: "unstr_lookup e a x = Some v \<Longrightarrow> lookup cd pc = Some (Lookup\<^sub>b y) \<Longrightarrow> x \<le> y \<Longrightarrow> 
   pc < length cd \<Longrightarrow> a \<le> ep \<Longrightarrow> restructurable_env e ep hp \<Longrightarrow> iter_evala (assemble_code cd) 
     (5 + 2 * x) (AS (case_register h (assemble_env e ep) vs sh) (case_register hp ep vp sp) a 
-      (Reg Env) (5 + 2 * x + assembly_map cd pc)) = Some (AS (case_register h (assemble_env e ep)
-        (vs(vp := (Reg Hp, v))) sh) (case_register hp ep (Suc vp) sp) 0 (Con 0) 
+      (Some Env) (5 + 2 * x + assembly_map cd pc)) = Some (AS (case_register h (assemble_env e ep)
+        (vs(vp := (Some Hp, v))) sh) (case_register hp ep (Suc vp) sp) 0 None
           (assembly_map cd pc))"
 proof (induction e a x rule: unstr_lookup.induct)
   case (3 e p)
   moreover from 3 have "lookup (assemble_code cd) (4 + assembly_map cd pc) = 
     Some (ASub (Acc (Reg Env)) 2)" by simp
   moreover from 3 have "lookup (assemble_code cd) (3 + assembly_map cd pc) = 
-    Some (AGet (Acc (Reg Env)) (Reg Hp))" by simp
+    Some (AGet (Acc (Reg Env)))" by simp
   moreover from 3 have "lookup (assemble_code cd) (2 + assembly_map cd pc) = 
-    Some (APut Vals (Acc (Con 0)))" by (simp del: add_2_eq_Suc)
+    Some (APut Vals (Acc (Reg Hp)))" by (simp del: add_2_eq_Suc)
   ultimately show ?case by (simp add: numeral_def assemble_env_def split: if_splits)
 next
   case (4 e p x)
   moreover hence "lookup (assemble_code cd) (6 + 2 * x + assembly_map cd pc) = 
     Some (ASub (Acc (Reg Env)) (Suc 0))" by simp
   moreover from 4 have "lookup (assemble_code cd) (5 + 2 * x + assembly_map cd pc) = 
-    Some (AGet (Acc (Reg Env)) (Reg Env))" by simp
+    Some (AGet (Acc (Reg Env)))" by simp
   ultimately have X: "iter_evala (assemble_code cd) 2 (AS (case_register h (assemble_env e ep) vs 
-    sh) (case_register hp ep vp sp) (Suc (Suc p)) (Reg Env)
+    sh) (case_register hp ep vp sp) (Suc (Suc p)) (Some Env)
       (7 + 2 * x + assembly_map cd pc)) = Some (AS (case_register h (assemble_env e ep) vs sh) 
-        (case_register hp ep vp sp) (e (Suc p)) (Reg Env) (5 + 2 * x + assembly_map cd pc))" 
+        (case_register hp ep vp sp) (e (Suc p)) (Some Env) (5 + 2 * x + assembly_map cd pc))" 
     by (simp add: numeral_def assemble_env_def split: if_splits) presburger
   from 4 have "Suc p < ep" and "even p" and "restructurable_env e ep hp" by (auto split: if_splits)
   hence "e (Suc p) < ep" by (auto split: if_splits)
   moreover with 4 have "iter_evala (assemble_code cd) (5 + 2 * x)
-    (AS (case_register h (assemble_env e ep) vs sh) (case_register hp ep vp sp) (e (Suc p)) (Reg Env)
+    (AS (case_register h (assemble_env e ep) vs sh) (case_register hp ep vp sp) (e (Suc p)) (Some Env)
       (5 + 2 * x + assembly_map cd pc)) = Some (AS (case_register h (assemble_env e ep) 
-        (vs(vp := (Reg Hp, v))) sh) (case_register hp ep (Suc vp) sp) 0 (Con 0) 
+        (vs(vp := (Some Hp, v))) sh) (case_register hp ep (Suc vp) sp) 0 None
           (assembly_map cd pc))" by (simp split: if_splits)
   with X have "iter_evala (assemble_code cd) (2 + (5 + 2 * x))
     (AS (case_register h (assemble_env e ep) vs sh) (case_register hp ep vp sp) (Suc (Suc p)) (
-      Reg Env) (7 + 2 * x + assembly_map cd pc)) = Some (AS (case_register h (assemble_env e ep) 
-        (vs(vp := (Reg Hp, v))) sh) (case_register hp ep (Suc vp) sp) 0 (Con 0) 
+      Some Env) (7 + 2 * x + assembly_map cd pc)) = Some (AS (case_register h (assemble_env e ep) 
+        (vs(vp := (Some Hp, v))) sh) (case_register hp ep (Suc vp) sp) 0 None
           (assembly_map cd pc))" 
     using iter_evala_combine by blast
   thus ?case by simp
@@ -411,35 +411,35 @@ proof (induction cd\<^sub>b \<Sigma>\<^sub>u \<Sigma>\<^sub>u' rule: eval\<^sub>
   moreover from ev\<^sub>u_lookup have "lookup (assemble_code cd) (6 + 2 * x + assembly_map cd pc) = 
     Some (ASub (Acc (Reg Stk)) 1)" by simp
   moreover from ev\<^sub>u_lookup have "lookup (assemble_code cd) (5 + 2 * x + assembly_map cd pc) = 
-    Some (AGet (Acc (Reg Stk)) (Reg Env))" by simp
+    Some (AGet (Acc (Reg Stk)))" by simp
   ultimately have X: "iter_evala (assemble_code cd) 3 
     (AS (case_register (assm_hp cd h hp) (assemble_env e ep) (assemble_vals vs vp) 
-      (assm_stk cd sh (Suc sp))) (case_register hp ep vp (Suc sp)) 0 (Con 0) 
+      (assm_stk cd sh (Suc sp))) (case_register hp ep vp (Suc sp)) 0 None
         (8 + 2 * x + assembly_map cd pc)) = Some (AS (case_register (assm_hp cd h hp) 
           (assemble_env e ep) (assemble_vals vs vp) (assm_stk cd sh (Suc sp))) 
-            (case_register hp ep vp (Suc sp)) (sh sp) (Reg Env) (5 + 2 * x + assembly_map cd pc))" 
+            (case_register hp ep vp (Suc sp)) (sh sp) (Some Env) (5 + 2 * x + assembly_map cd pc))" 
     by (simp add: numeral_def)
   from ev\<^sub>u_lookup have "sh sp \<le> ep" by auto
   with ev\<^sub>u_lookup have "iter_evala (assemble_code cd) (5 + 2 * x) 
     (AS (case_register (assm_hp cd h hp) (assemble_env e ep) (assemble_vals vs vp) 
-      (assm_stk cd sh (Suc sp))) (case_register hp ep vp (Suc sp)) (sh sp) (Reg Env) 
+      (assm_stk cd sh (Suc sp))) (case_register hp ep vp (Suc sp)) (sh sp) (Some Env) 
         (5 + 2 * x + assembly_map cd pc)) = Some (AS (case_register (assm_hp cd h hp) 
           (assemble_env e ep) (assemble_vals (vs(vp := y)) (Suc vp)) (assm_stk cd sh (Suc sp))) 
-            (case_register hp ep (Suc vp) (Suc sp)) 0 (Con 0) (assembly_map cd pc))" 
+            (case_register hp ep (Suc vp) (Suc sp)) 0 None (assembly_map cd pc))" 
     by simp
   with X have "iter_evala (assemble_code cd) (3 + (5 + 2 * x)) 
     (AS (case_register (assm_hp cd h hp) (assemble_env e ep) (assemble_vals vs vp) 
-      (assm_stk cd sh (Suc sp))) (case_register hp ep vp (Suc sp)) 0 (Con 0) 
+      (assm_stk cd sh (Suc sp))) (case_register hp ep vp (Suc sp)) 0 None
         (8 + 2 * x + assembly_map cd pc)) = Some (AS (case_register (assm_hp cd h hp) 
           (assemble_env e ep) (assemble_vals (vs(vp := y)) (Suc vp)) (assm_stk cd sh (Suc sp))) 
-            (case_register hp ep (Suc vp) (Suc sp)) 0 (Con 0) (assembly_map cd pc))" 
+            (case_register hp ep (Suc vp) (Suc sp)) 0 None (assembly_map cd pc))" 
     using iter_evala_combine by blast
   hence "iter_evala (assemble_code cd) (3 + (5 + 2 * x)) 
     (AS (case_register (assm_hp cd h hp) (assemble_env e ep) (assemble_vals vs vp) 
-      (assm_stk cd sh (Suc sp))) (case_register hp ep vp (Suc sp)) 0 (Con 0) 
+      (assm_stk cd sh (Suc sp))) (case_register hp ep vp (Suc sp)) 0 None
         (8 + (2 * x + assembly_map cd pc))) = Some (AS (case_register (assm_hp cd h hp) 
           (assemble_env e ep) (assemble_vals (vs(vp := y)) (Suc vp)) (assm_stk cd sh (Suc sp))) 
-            (case_register hp ep (Suc vp) (Suc sp)) 0 (Con 0) (assembly_map cd pc))"
+            (case_register hp ep (Suc vp) (Suc sp)) 0 None (assembly_map cd pc))"
     by (simp add: add.assoc)
   with ev\<^sub>u_lookup show ?case by auto
 next
@@ -458,11 +458,11 @@ next
     Some (AAdd (Reg Hp) 1)" by (simp del: add_2_eq_Suc)
   ultimately have "iter_evala (assemble_code cd) 8 (AS (case_register (assm_hp cd h hp) 
     (assemble_env e ep) (assemble_vals vs vp) (assm_stk cd sh (Suc sp))) 
-      (case_register hp ep vp (Suc sp)) 0 (Con 0) (assembly_map cd (Suc pc))) = Some (AS 
+      (case_register hp ep vp (Suc sp)) 0 None (assembly_map cd (Suc pc))) = Some (AS 
         (case_register (assm_hp cd (h(hp := (PConst, Suc 0), Suc hp := (PConst, k), 
           Suc (Suc hp) := (PConst, 0))) (3 + hp)) (assemble_env e ep) (assemble_vals (vs(vp := hp)) 
             (Suc vp)) (assm_stk cd sh (Suc sp))) (case_register (3 + hp) ep (Suc vp) (Suc sp)) 0 
-              (Con 0) (assembly_map cd pc))" 
+              None (assembly_map cd pc))" 
     by (auto simp add: numeral_def)
   thus ?case by auto
 next
@@ -476,24 +476,24 @@ next
   moreover from ev\<^sub>u_pushlam have "lookup (assemble_code cd) (8 + assembly_map cd pc) = 
     Some (ASub (Acc (Reg Stk)) 1)" by simp
   moreover from ev\<^sub>u_pushlam have "lookup (assemble_code cd) (7 + assembly_map cd pc) = 
-    Some (AGet (Acc (Reg Stk)) (Reg Env))" by simp
+    Some (AGet (Acc (Reg Stk)))" by simp
   moreover from ev\<^sub>u_pushlam have "lookup (assemble_code cd) (6 + assembly_map cd pc) = 
     Some (APut Hp (Con 0))" by simp
   moreover from ev\<^sub>u_pushlam have "lookup (assemble_code cd) (5 + assembly_map cd pc) = 
     Some (AAdd (Reg Hp) 1)" by simp
   moreover from ev\<^sub>u_pushlam have "lookup (assemble_code cd) (4 + assembly_map cd pc) =
-    Some (APut Hp (Acc (Con 0)))" by simp
+    Some (APut Hp (Acc (Reg Env)))" by simp
   moreover from ev\<^sub>u_pushlam have "lookup (assemble_code cd) (3 + assembly_map cd pc) = 
     Some (AAdd (Reg Hp) 1)" by simp
   moreover from ev\<^sub>u_pushlam have "lookup (assemble_code cd) (2 + assembly_map cd pc) = 
     Some (AMov (Con 0))" by (simp del: add_2_eq_Suc)
   ultimately have "iter_evala (assemble_code cd) 12 (AS (case_register (assm_hp cd h hp) 
     (assemble_env e ep) (assemble_vals vs vp) (assm_stk cd sh (Suc sp))) 
-      (case_register hp ep vp (Suc sp)) 0 (Con 0) (assembly_map cd (Suc pc))) = Some (AS 
+      (case_register hp ep vp (Suc sp)) 0 None (assembly_map cd (Suc pc))) = Some (AS 
         (case_register (assm_hp cd (h(hp := (PConst, 0), Suc hp := (PEnv, sh sp), 
           Suc (Suc hp) := (PCode, pc'))) (3 + hp)) (assemble_env e ep) (assemble_vals (vs(vp := hp)) 
             (Suc vp)) (assm_stk cd sh (Suc sp))) (case_register (3 + hp) ep (Suc vp) (Suc sp)) 0 
-              (Con 0) (assembly_map cd pc))" 
+              None (assembly_map cd pc))" 
     by (auto simp add: numeral_def)
   thus ?case by auto
 next
@@ -502,11 +502,11 @@ next
   moreover from ev\<^sub>u_apply have "lookup (assemble_code cd) (23 + assembly_map cd pc) = 
     Some (ASub (Reg Vals) 1)" by simp
   moreover from ev\<^sub>u_apply have "lookup (assemble_code cd) (22 + assembly_map cd pc) = 
-    Some (AGet (Reg Vals) (Reg Hp))" by simp
+    Some (AGet (Reg Vals))" by simp
   moreover from ev\<^sub>u_apply have "lookup (assemble_code cd) (21 + assembly_map cd pc) = 
     Some (APut Vals (Con 0))" by simp
   moreover from ev\<^sub>u_apply have "lookup (assemble_code cd) (20 + assembly_map cd pc) = 
-    Some (APut Env (Acc (Con 0)))" by simp
+    Some (APut Env (Acc (Reg Hp)))" by simp
   moreover from ev\<^sub>u_apply have "lookup (assemble_code cd) (19 + assembly_map cd pc) = 
     Some (AAdd (Reg Env) 1)" by simp
   moreover from ev\<^sub>u_apply have "lookup (assemble_code cd) (18 + assembly_map cd pc) = 
@@ -514,7 +514,7 @@ next
   moreover from ev\<^sub>u_apply have "lookup (assemble_code cd) (17 + assembly_map cd pc) = 
     Some (ASub (Acc (PC 0)) 18)" by simp
   moreover from ev\<^sub>u_apply have "lookup (assemble_code cd) (16 + assembly_map cd pc) = 
-    Some (APut Stk (Acc (Con 0)))" by simp
+    Some (APut Stk (Acc (PC 0)))" by simp
   moreover from ev\<^sub>u_apply have "lookup (assemble_code cd) (15 + assembly_map cd pc) = 
     Some (AAdd (Reg Stk) 1)" by simp
   moreover from ev\<^sub>u_apply have "lookup (assemble_code cd) (14 + assembly_map cd pc) = 
@@ -522,34 +522,34 @@ next
   moreover from ev\<^sub>u_apply have "lookup (assemble_code cd) (13 + assembly_map cd pc) = 
     Some (AAdd (Acc (Reg Env)) 1)" by simp
   moreover from ev\<^sub>u_apply have "lookup (assemble_code cd) (12 + assembly_map cd pc) = 
-    Some (APut Stk (Acc (Con 0)))" by simp
+    Some (APut Stk (Acc (Reg Env)))" by simp
   moreover from ev\<^sub>u_apply have "lookup (assemble_code cd) (11 + assembly_map cd pc) = 
     Some (AAdd (Reg Stk) 1)" by simp
   moreover from ev\<^sub>u_apply have "lookup (assemble_code cd) (10 + assembly_map cd pc) = 
     Some (ASub (Reg Vals) 1)" by simp
   moreover from ev\<^sub>u_apply have "lookup (assemble_code cd) (9 + assembly_map cd pc) = 
-    Some (AGet (Reg Vals) (Reg Hp))" by simp
+    Some (AGet (Reg Vals))" by simp
   moreover from ev\<^sub>u_apply have "lookup (assemble_code cd) (8 + assembly_map cd pc) = 
     Some (AAdd (Acc (Reg Hp)) 1)" by simp
   moreover from ev\<^sub>u_apply have "lookup (assemble_code cd) (7 + assembly_map cd pc) = 
-    Some (AGet (Acc (Reg Hp)) (Reg Env))" by simp
+    Some (AGet (Acc (Reg Hp)))" by simp
   moreover from ev\<^sub>u_apply have "lookup (assemble_code cd) (6 + assembly_map cd pc) = 
-    Some (APut Env (Acc (Con 0)))" by simp
+    Some (APut Env (Acc (Reg Env)))" by simp
   moreover from ev\<^sub>u_apply have "lookup (assemble_code cd) (5 + assembly_map cd pc) = 
     Some (AAdd (Reg Env) 1)" by simp
   moreover from ev\<^sub>u_apply have "lookup (assemble_code cd) (4 + assembly_map cd pc) = 
-    Some (AGet (Reg Vals) (Reg Hp))" by simp
+    Some (AGet (Reg Vals))" by simp
   moreover from ev\<^sub>u_apply have "lookup (assemble_code cd) (3 + assembly_map cd pc) = 
     Some (APut Vals (Con 0))" by simp
   moreover from ev\<^sub>u_apply have "lookup (assemble_code cd) (2 + assembly_map cd pc) = 
     Some (AAdd (Acc (Reg Hp)) 2)" by (simp del: add_2_eq_Suc)
   ultimately have "iter_evala (assemble_code cd) 24 (AS (case_register (assm_hp cd h hp) 
     (assemble_env e ep) (assemble_vals vs (Suc (Suc vp))) (assm_stk cd sh (Suc sp))) 
-      (case_register hp ep (Suc (Suc vp)) (Suc sp)) 0 (Con 0) (assembly_map cd (Suc pc))) = 
+      (case_register hp ep (Suc (Suc vp)) (Suc sp)) 0 None (assembly_map cd (Suc pc))) = 
         Some (AS (case_register (assm_hp cd h hp) (assemble_env (e(ep := vs (Suc vp), 
           Suc ep := snd (h (Suc (vs vp))))) (Suc (Suc ep))) (assemble_vals vs vp) 
             (assm_stk cd (sh(Suc sp := pc, Suc (Suc sp) := Suc (Suc ep))) (Suc (Suc (Suc sp))))) 
-              (case_register hp (Suc (Suc ep)) vp (Suc (Suc (Suc sp)))) 0 (Con 0) 
+              (case_register hp (Suc (Suc ep)) vp (Suc (Suc (Suc sp)))) 0 None
                 (assembly_map cd (snd (h (Suc (Suc (vs vp)))))))"
     by (auto simp add: numeral_def assemble_vals_def)
   thus ?case by auto
@@ -562,12 +562,12 @@ next
   moreover from ev\<^sub>u_return have "lookup (assemble_code cd) (3 + assembly_map cd pc) = 
     Some (ASub (Reg Stk) 1)" by simp
   moreover from ev\<^sub>u_return have "lookup (assemble_code cd) (2 + assembly_map cd pc) = 
-    Some (AGet (Reg Stk) (PC 0))" by (simp del: add_2_eq_Suc)
+    Some (AGet (Reg Stk))" by (simp del: add_2_eq_Suc)
   ultimately have "iter_evala (assemble_code cd) 6 (AS (case_register (assm_hp cd h hp) 
     (assemble_env e ep) (assemble_vals vs vp) (assm_stk cd sh (Suc (Suc sp)))) 
-      (case_register hp ep vp (Suc (Suc sp))) 0 (Con 0) (assembly_map cd (Suc pc))) = 
+      (case_register hp ep vp (Suc (Suc sp))) 0 None (assembly_map cd (Suc pc))) = 
         Some (AS (case_register (assm_hp cd h hp) (assemble_env e ep) (assemble_vals vs vp) 
-          (assm_stk cd sh sp)) (case_register hp ep vp sp) 0 (Con 0) (assembly_map cd (sh sp)))"
+          (assm_stk cd sh sp)) (case_register hp ep vp sp) 0 None (assembly_map cd (sh sp)))"
     by (simp add: numeral_def split: prod.splits)
   thus ?case by auto
 next
@@ -576,11 +576,11 @@ next
   moreover from ev\<^sub>u_jump have "lookup (assemble_code cd) (20 + assembly_map cd pc) = 
     Some (ASub (Reg Vals) 1)" by simp
   moreover from ev\<^sub>u_jump have "lookup (assemble_code cd) (19 + assembly_map cd pc) = 
-    Some (AGet (Reg Vals) (Reg Hp))" by simp
+    Some (AGet (Reg Vals))" by simp
   moreover from ev\<^sub>u_jump have "lookup (assemble_code cd) (18 + assembly_map cd pc) = 
     Some (APut Vals (Con 0))" by simp
   moreover from ev\<^sub>u_jump have "lookup (assemble_code cd) (17 + assembly_map cd pc) = 
-    Some (APut Env (Acc (Con 0)))" by simp
+    Some (APut Env (Acc (Reg Hp)))" by simp
   moreover from ev\<^sub>u_jump have "lookup (assemble_code cd) (16 + assembly_map cd pc) = 
     Some (AAdd (Reg Env) 1)" by simp
   moreover from ev\<^sub>u_jump have "lookup (assemble_code cd) (15 + assembly_map cd pc) = 
@@ -590,34 +590,34 @@ next
   moreover from ev\<^sub>u_jump have "lookup (assemble_code cd) (13 + assembly_map cd pc) = 
     Some (ASub (Reg Stk) 1)" by simp
   moreover from ev\<^sub>u_jump have "lookup (assemble_code cd) (12 + assembly_map cd pc) = 
-    Some (APut Stk (Acc (Con 0)))" by simp
+    Some (APut Stk (Acc (Reg Env)))" by simp
   moreover from ev\<^sub>u_jump have "lookup (assemble_code cd) (11 + assembly_map cd pc) =
     Some (AAdd (Reg Stk) 1)" by simp
   moreover from ev\<^sub>u_jump have "lookup (assemble_code cd) (10 + assembly_map cd pc) = 
     Some (ASub (Reg Vals) 1)" by simp
   moreover from ev\<^sub>u_jump have "lookup (assemble_code cd) (9 + assembly_map cd pc) = 
-    Some (AGet (Reg Vals) (Reg Hp))" by simp
+    Some (AGet (Reg Vals))" by simp
   moreover from ev\<^sub>u_jump have "lookup (assemble_code cd) (8 + assembly_map cd pc) = 
     Some (AAdd (Acc (Reg Hp)) 1)" by simp
   moreover from ev\<^sub>u_jump have "lookup (assemble_code cd) (7 + assembly_map cd pc) = 
-    Some (AGet (Acc (Reg Hp)) (Reg Env))" by simp
+    Some (AGet (Acc (Reg Hp)))" by simp
   moreover from ev\<^sub>u_jump have "lookup (assemble_code cd) (6 + assembly_map cd pc) = 
-    Some (APut Env (Acc (Con 0)))" by simp
+    Some (APut Env (Acc (Reg Env)))" by simp
   moreover from ev\<^sub>u_jump have "lookup (assemble_code cd) (5 + assembly_map cd pc) = 
     Some (AAdd (Reg Env) 1)" by simp
   moreover from ev\<^sub>u_jump have "lookup (assemble_code cd) (4 + assembly_map cd pc) = 
-    Some (AGet (Reg Vals) (Reg Hp))" by simp
+    Some (AGet (Reg Vals))" by simp
   moreover from ev\<^sub>u_jump have "lookup (assemble_code cd) (3 + assembly_map cd pc) = 
     Some (APut Vals (Con 0))" by simp
   moreover from ev\<^sub>u_jump have "lookup (assemble_code cd) (2 + assembly_map cd pc) = 
     Some (AAdd (Acc (Reg Hp)) 2)" by (simp del: add_2_eq_Suc)
   ultimately have "iter_evala (assemble_code cd) 21 (AS (case_register (assm_hp cd h hp) 
     (assemble_env e ep) (assemble_vals vs (Suc (Suc vp))) (assm_stk cd sh (Suc sp))) 
-      (case_register hp ep (Suc (Suc vp)) (Suc sp)) 0 (Con 0) (assembly_map cd (Suc pc))) = 
+      (case_register hp ep (Suc (Suc vp)) (Suc sp)) 0 None (assembly_map cd (Suc pc))) = 
         Some (AS (case_register (assm_hp cd h hp) (assemble_env (e(ep := vs (Suc vp), 
           Suc ep := snd (h (Suc (vs vp))))) (Suc (Suc ep))) (assemble_vals vs vp) 
             (assm_stk cd (sh(sp := Suc (Suc ep))) (Suc sp))) (case_register hp 
-              (Suc (Suc ep)) vp (Suc sp)) 0 (Con 0) (assembly_map cd (snd (h (Suc (Suc (vs vp)))))))"
+              (Suc (Suc ep)) vp (Suc sp)) 0 None (assembly_map cd (snd (h (Suc (Suc (vs vp)))))))"
     by (auto simp add: numeral_def assemble_vals_def)
   thus ?case by auto
 qed
@@ -654,17 +654,17 @@ qed
 (* We no longer do the reverse (completeness) direction because it's rather complex to even state 
 now *)
 
-lemma [simp]: "assm_hp cd h 0 = (\<lambda>x. (Con 0, 0))"
+lemma [simp]: "assm_hp cd h 0 = (\<lambda>x. (None, 0))"
   by rule (simp add: assemble_heap_def)
 
-lemma [simp]: "assemble_env e 0 = (\<lambda>x. (Con 0, 0))"
+lemma [simp]: "assemble_env e 0 = (\<lambda>x. (None, 0))"
   by rule (simp add: assemble_env_def)
 
-lemma [simp]: "assemble_vals vs 0 = (\<lambda>x. (Con 0, 0))"
+lemma [simp]: "assemble_vals vs 0 = (\<lambda>x. (None, 0))"
   by rule (simp add: assemble_vals_def)
 
 lemma [simp]: "assm_stk cd (mp(0 := a, Suc 0 := b)) 2 = 
-    (\<lambda>x. (Con 0, 0))(0 := (PC 0, assembly_map cd a), Suc 0 := (Reg Env, b))"
+    (\<lambda>x. (None, 0))(0 := (None, assembly_map cd a), Suc 0 := (Some Env, b))"
   by rule (simp add: assemble_stack_def)
 
 lemma [simp]: "
