13MachineCode/Disassemble.thy
@@ -20,21 +20,19 @@ primrec pseudoreg_size :: "pseudoreg \<Rightarrow> nat" where
 | "pseudoreg_size (Con k) = 1"
 | "pseudoreg_size (Acc _) = 1"
 
-fun pseudoreg_map :: "pseudoreg \<times> nat \<Rightarrow> nat" where
-  "pseudoreg_map (Reg r, x) = 4 * x + register_offset r"
-| "pseudoreg_map (PC _, x) = x"
-| "pseudoreg_map (Con k, x) = x"
-| "pseudoreg_map (Acc _, x) = x"
+fun pseudoreg_map :: "register option \<times> nat \<Rightarrow> nat" where
+  "pseudoreg_map (Some r, x) = 4 * x + register_offset r"
+| "pseudoreg_map (None, x) = x"
 
 fun disassemble' :: "assm \<Rightarrow> mach" where
   "disassemble' (AMov (Reg r)) = MOV R5 (register_map r)"
 | "disassemble' (AMov (PC _)) = MVP R5"
 | "disassemble' (AMov (Con k)) = LDI R5 k"
 | "disassemble' (AMov (Acc _)) = undefined"
-| "disassemble' (AGet (Reg r) t) = LOD R5 (register_map r)"
-| "disassemble' (AGet (PC _) t) = undefined"
-| "disassemble' (AGet (Con k) t) = undefined"
-| "disassemble' (AGet (Acc r) t) = LOD R5 R5"
+| "disassemble' (AGet (Reg r)) = LOD R5 (register_map r)"
+| "disassemble' (AGet (PC _)) = undefined"
+| "disassemble' (AGet (Con k)) = undefined"
+| "disassemble' (AGet (Acc r)) = LOD R5 R5"
 | "disassemble' (APut r (Reg r')) = STO (register_map r) (register_map r')"
 | "disassemble' (APut r (PC k)) = STI (register_map r) k"
 | "disassemble' (APut r (Con k)) = STI (register_map r) k"
@@ -59,10 +57,10 @@ fun unmap_mem' :: "nat \<Rightarrow> register \<times> nat" where
 | "unmap_mem' (Suc (Suc (Suc 0))) = (Stk, 0)"
 | "unmap_mem' (Suc (Suc (Suc (Suc x)))) = (case unmap_mem' x of (a, b) \<Rightarrow> (a, Suc b))"
 
-definition unmap_mem :: "(register \<Rightarrow> nat \<Rightarrow> pseudoreg \<times> nat) \<Rightarrow> nat \<Rightarrow> nat" where
+definition unmap_mem :: "(register \<Rightarrow> nat \<Rightarrow> register option \<times> nat) \<Rightarrow> nat \<Rightarrow> nat" where
   "unmap_mem m x = (case unmap_mem' x of (r, p) \<Rightarrow> pseudoreg_map (m r p))"
 
-primrec inv_register_map :: "(register \<Rightarrow> nat) \<Rightarrow> nat \<Rightarrow> pseudoreg \<Rightarrow> reg \<Rightarrow> nat" where
+primrec inv_register_map :: "(register \<Rightarrow> nat) \<Rightarrow> nat \<Rightarrow> register option \<Rightarrow> reg \<Rightarrow> nat" where
   "inv_register_map rs a t R1 = rs Hp * 4"
 | "inv_register_map rs a t R2 = rs Env * 4 + 1"
 | "inv_register_map rs a t R3 = rs Vals * 4 + 2"
@@ -122,28 +120,21 @@ qed
 
 lemma inv_reg_map_reg: "
   (inv_register_map ps a act)(R5 := inv_register_map ps a act (register_map r)) = 
-    inv_register_map ps (ps r) (Reg r)"
+    inv_register_map ps (ps r) (Some r)"
 proof
   fix x
   show "((inv_register_map ps a act)(R5 := inv_register_map ps a act (register_map r))) x = 
-      inv_register_map ps (ps r) (Reg r) x"
+      inv_register_map ps (ps r) (Some r) x"
   proof (induction x)
     case R5
     thus ?case by (induction r) simp_all
   qed simp_all
 qed
 
-lemma inv_reg_map_pc: "(inv_register_map ps a act)(R5 := pc) = inv_register_map ps pc (PC 0)"
+lemma inv_reg_map_none: "(inv_register_map ps a act)(R5 := k) = inv_register_map ps k None"
 proof
   fix x
-  show "((inv_register_map ps a act)(R5 := pc)) x = inv_register_map ps pc (PC 0) x"
-    by (induction x) simp_all
-qed
-
-lemma inv_reg_map_con: "(inv_register_map ps a act)(R5 := k) = inv_register_map ps k (Con 0)"
-proof
-  fix x
-  show "((inv_register_map ps a act)(R5 := k)) x = inv_register_map ps k (Con 0) x"
+  show "((inv_register_map ps a act)(R5 := k)) x = inv_register_map ps k None x"
     by (induction x) simp_all
 qed
 
@@ -179,15 +170,17 @@ proof
     by (induction x) auto
 qed
 
-lemma [simp]: "(inv_register_map ps a act) (R5 := pseudoreg_map (act, a) + pseudoreg_size act * k) = 
-  inv_register_map ps (a + k) act"
+lemma [simp]: "match_regs act t \<Longrightarrow>
+  (inv_register_map ps a act) (R5 := pseudoreg_map (act, a) + pseudoreg_size t * k) = 
+    inv_register_map ps (a + k) act"
 proof
   fix x
-  show "((inv_register_map ps a act) (R5 := pseudoreg_map (act, a) + pseudoreg_size act * k)) x =
+  assume "match_regs act t"
+  thus "((inv_register_map ps a act) (R5 := pseudoreg_map (act, a) + pseudoreg_size t * k)) x =
     inv_register_map ps (a + k) act x" 
   proof (induction x)
     case R5
-    thus ?case by (induction act) simp_all
+    thus ?case by (induction act t rule: match_regs.induct) simp_all
   qed simp_all
 qed
 
@@ -203,31 +196,24 @@ proof
     by (induction x) auto
 qed
 
-lemma [simp]: "a \<ge> k \<Longrightarrow> 
-  (inv_register_map ps a act) (R5 := pseudoreg_map (act, a) - pseudoreg_size act * k) = 
+lemma [simp]: "a \<ge> k \<Longrightarrow> match_regs act t \<Longrightarrow>
+  (inv_register_map ps a act) (R5 := pseudoreg_map (act, a) - pseudoreg_size t * k) = 
     inv_register_map ps (a - k) act"
 proof
   fix x
-  assume "a \<ge> k"
+  assume "a \<ge> k" and "match_regs act t"
   thus "((inv_register_map ps a act)
-    (R5 := pseudoreg_map (act, a) - pseudoreg_size act * k)) x =
+    (R5 := pseudoreg_map (act, a) - pseudoreg_size t * k)) x =
       inv_register_map ps (a - k) act x" 
   proof (induction x)
     case R5
-    thus ?case by (induction act) simp_all
+    thus ?case by (induction act t rule: match_regs.induct) simp_all
   qed simp_all
 qed
 
-lemma [simp]: "unmap_mem mem (inv_register_map ps a (Reg r) (register_map r)) = 
+lemma [simp]: "unmap_mem mem (inv_register_map ps a (Some r) (register_map r)) = 
     pseudoreg_map (mem r (ps r))"
   by (induction r) (simp_all add: unmap_mem_def split: prod.splits)
-
-lemma [simp]: "((inv_register_map ps a (PC 0))(R5 := 0)) = inv_register_map ps 0 (Con 0)"
-proof
-  fix x
-  show "((inv_register_map ps a (PC 0))(R5 := 0)) x = inv_register_map ps 0 (Con 0) x" 
-    by (induction x) simp_all
-qed
 
 lemma [simp]: "mem r (ps r) = (t, b) \<Longrightarrow> 
   (inv_register_map ps a act)(R5 := unmap_mem mem (inv_register_map ps a act (register_map r))) = 
@@ -244,31 +230,17 @@ proof
 qed
 
 lemma unmap_upd_k: "(unmap_mem mem)(inv_register_map ps a act (register_map r) := k) = 
-  unmap_mem (mem_upd mem r (ps r) (Con 0, k))"
-proof
-  fix x
-  show "((unmap_mem mem)(inv_register_map ps a act (register_map r) := k)) x =
-      unmap_mem (mem_upd mem r (ps r) (Con 0, k)) x"
-    by (induction r) (auto simp add: unmap_mem_def split: prod.splits)
-qed
-
-lemma unmap_upd_pc: "(unmap_mem mem)(inv_register_map ps a act (register_map r) := k) = 
-  unmap_mem (mem_upd mem r (ps r) (PC 0, k))"
-proof
-  fix x
-  show "((unmap_mem mem)(inv_register_map ps a act (register_map r) := k)) x =
-      unmap_mem (mem_upd mem r (ps r) (PC 0, k)) x"
-    by (induction r) (auto simp add: unmap_mem_def split: prod.splits)
-qed
+  unmap_mem (mem_upd mem r (ps r) (None, k))"
+  by (rule, induction r) (auto simp add: unmap_mem_def split: prod.splits)
 
 lemma [simp]: "((unmap_mem mem)
   (inv_register_map ps a act (register_map r) := inv_register_map ps a act (register_map r'))) = 
-    unmap_mem (mem_upd mem r (ps r) (Reg r', ps r'))"
+    unmap_mem (mem_upd mem r (ps r) (Some r', ps r'))"
 proof
   fix x
   show "((unmap_mem mem)
     (inv_register_map ps a act (register_map r) := inv_register_map ps a act (register_map r'))) x = 
-      unmap_mem (mem_upd mem r (ps r) (Reg r', ps r')) x"
+      unmap_mem (mem_upd mem r (ps r) (Some r', ps r')) x"
   proof (induction r)
     case Hp
     thus ?case by (induction r') (auto simp add: unmap_mem_def split: prod.splits)
@@ -294,12 +266,12 @@ proof
 qed
 
 lemma [simp]: "mem m a = (t, b) \<Longrightarrow>  
-  ((inv_register_map ps a (Reg m))(R5 := unmap_mem mem (4 * a + register_offset m))) = 
+  ((inv_register_map ps a (Some m))(R5 := unmap_mem mem (4 * a + register_offset m))) = 
     inv_register_map ps b t"
 proof 
   fix x
   assume "mem m a = (t, b)"
-  thus "((inv_register_map ps a (Reg m))(R5 := unmap_mem mem (4 * a + register_offset m))) 
+  thus "((inv_register_map ps a (Some m))(R5 := unmap_mem mem (4 * a + register_offset m))) 
     x = inv_register_map ps b t x"
       by (induction x) (auto simp add: unmap_mem_def)
 qed
@@ -322,32 +294,32 @@ next
   case (eva_movp cd pc x mem ps a act)
   hence "disassemble cd \<tturnstile> MS (inv_register_map ps a act) (unmap_mem mem) (Suc pc) \<leadsto>\<^sub>m
     MS ((inv_register_map ps a act)(R5 := pc)) (unmap_mem mem) pc" by simp
-  thus ?case by (simp add: inv_reg_map_pc)
+  thus ?case by (simp add: inv_reg_map_none)
 next
   case (eva_movk cd pc k mem ps a act)
   hence "disassemble cd \<tturnstile> MS (inv_register_map ps a act) (unmap_mem mem) (Suc pc) \<leadsto>\<^sub>m
     MS ((inv_register_map ps a act)(R5 := k)) (unmap_mem mem) pc" by simp
-  thus ?case by (simp add: inv_reg_map_con)
+  thus ?case by (simp add: inv_reg_map_none)
 next
-  case (eva_geta cd pc m t mem a b ps) 
+  case (eva_geta cd pc m mem a t b ps) 
   hence "disassemble cd ! pc = LOD R5 R5" by simp
-  hence "disassemble cd \<tturnstile> MS (inv_register_map ps a (Reg m)) (unmap_mem mem) (Suc pc) \<leadsto>\<^sub>m 
-    MS ((inv_register_map ps a (Reg m))(R5 := unmap_mem mem (inv_register_map ps a (Reg m) R5))) 
+  hence "disassemble cd \<tturnstile> MS (inv_register_map ps a (Some m)) (unmap_mem mem) (Suc pc) \<leadsto>\<^sub>m 
+    MS ((inv_register_map ps a (Some m))(R5 := unmap_mem mem (inv_register_map ps a (Some m) R5))) 
       (unmap_mem mem) pc" by (metis evm_lod)
   with eva_geta(2) show ?case by simp
 next
-  case (eva_get cd pc r t mem ps b a act)
+  case (eva_get cd pc r mem ps t b a act)
   hence "disassemble cd ! pc = LOD R5 (register_map r)" by simp
   hence "disassemble cd \<tturnstile> MS (inv_register_map ps a act) (unmap_mem mem) (Suc pc) \<leadsto>\<^sub>m
     MS ((inv_register_map ps a act)(R5 := (unmap_mem mem) ((inv_register_map ps a act) 
       (register_map r)))) (unmap_mem mem) pc" by (metis evm_lod)
   with eva_get(2) show ?case by simp
 next
-  case (eva_puta cd pc r x mem ps a act)
+  case (eva_puta cd pc r act mem ps a t)
   hence "disassemble cd ! pc = STO (register_map r) R5" by simp
-  hence "disassemble cd \<tturnstile> MS (inv_register_map ps a act) (unmap_mem mem) (Suc pc) \<leadsto>\<^sub>m
-    MS (inv_register_map ps a act) ((unmap_mem mem)(inv_register_map ps a act (register_map r) := 
-      inv_register_map ps a act R5)) pc" by (metis evm_sto)
+  hence "disassemble cd \<tturnstile> MS (inv_register_map ps a t) (unmap_mem mem) (Suc pc) \<leadsto>\<^sub>m
+    MS (inv_register_map ps a t) ((unmap_mem mem)(inv_register_map ps a t (register_map r) := 
+      inv_register_map ps a t R5)) pc" by (metis evm_sto)
   thus ?case by simp
 next
   case (eva_putp cd pc r k mem ps a act)
@@ -355,7 +327,7 @@ next
   hence "disassemble cd \<tturnstile> MS (inv_register_map ps a act) (unmap_mem mem) (Suc pc) \<leadsto>\<^sub>m 
     MS (inv_register_map ps a act) ((unmap_mem mem)((inv_register_map ps a act) (register_map r) := 
       k)) pc" by (metis evm_sti)
-  thus ?case by (simp add: unmap_upd_pc)
+  thus ?case by (simp add: unmap_upd_k)
 next
   case (eva_putr cd pc r r' mem ps a act)
   hence "disassemble cd ! pc = STO (register_map r) (register_map r')" by simp
@@ -371,55 +343,55 @@ next
       ((unmap_mem mem)(inv_register_map ps a act (register_map r) := k)) pc" by (metis evm_sti)
   thus ?case by (simp add: unmap_upd_k)
 next
-  case (eva_suba cd pc act k a mem ps)
-  hence "disassemble cd ! pc = SUB R5 (pseudoreg_size act * k)" by simp
+  case (eva_suba cd pc t k a act mem ps)
+  hence "disassemble cd ! pc = SUB R5 (pseudoreg_size t * k)" by simp
   hence "disassemble cd \<tturnstile> MS (inv_register_map ps a act) (unmap_mem mem) (Suc pc) \<leadsto>\<^sub>m 
-    MS ((inv_register_map ps a act)(R5 := inv_register_map ps a act R5 - pseudoreg_size act * k)) 
+    MS ((inv_register_map ps a act)(R5 := inv_register_map ps a act R5 - pseudoreg_size t * k)) 
       (unmap_mem mem) pc" by (metis evm_sub)
   with eva_suba show ?case by simp
 next
-  case (eva_adda cd pc act k mem ps a)
-  hence "disassemble cd ! pc = ADD R5 (pseudoreg_size act * k)" by simp
+  case (eva_adda cd pc t k act mem ps a)
+  hence "disassemble cd ! pc = ADD R5 (pseudoreg_size t * k)" by simp
   hence "disassemble cd \<tturnstile> MS (inv_register_map ps a act) (unmap_mem mem) (Suc pc) \<leadsto>\<^sub>m 
-    MS ((inv_register_map ps a act)(R5 := inv_register_map ps a act R5 + pseudoreg_size act * k)) 
+    MS ((inv_register_map ps a act)(R5 := inv_register_map ps a act R5 + pseudoreg_size t * k)) 
       (unmap_mem mem) pc" by (metis evm_add)
-  thus ?case by simp
+  with eva_adda show ?case by simp
 next
   case (eva_jmp cd pc mem ps a)
   hence "disassemble cd ! pc = JMP R5" by simp
-  hence "disassemble cd \<tturnstile> MS (inv_register_map ps a (PC 0)) (unmap_mem mem) (Suc pc) \<leadsto>\<^sub>m 
-    MS ((inv_register_map ps a (PC 0))(R5 := 0)) (unmap_mem mem) (inv_register_map ps a (PC 0) R5)" 
+  hence "disassemble cd \<tturnstile> MS (inv_register_map ps a None) (unmap_mem mem) (Suc pc) \<leadsto>\<^sub>m 
+    MS ((inv_register_map ps a None)(R5 := 0)) (unmap_mem mem) (inv_register_map ps a None R5)" 
       by (metis evm_jmp)
-  thus ?case by simp
+  thus ?case by (simp add: inv_reg_map_none)
 qed simp_all
 
 theorem correctm_iter [simp]: "iter (\<tturnstile> cd\<^sub>a \<leadsto>\<^sub>a) \<Sigma>\<^sub>a \<Sigma>\<^sub>a' \<Longrightarrow> 
     iter (\<tturnstile> disassemble cd\<^sub>a \<leadsto>\<^sub>m) (disassemble_state \<Sigma>\<^sub>a) (disassemble_state \<Sigma>\<^sub>a')"
   by (induction \<Sigma>\<^sub>a \<Sigma>\<^sub>a' rule: iter.induct) (simp, metis correctm iter_append iter_one)
  
-lemma [simp]: "inv_register_map (case_register 0 0 0 2) 0 (Con 0) = case_reg 0 1 2 11 0" 
+lemma [simp]: "inv_register_map (case_register 0 0 0 2) 0 None = case_reg 0 1 2 11 0" 
   by (auto split: reg.splits)
 
-lemma [simp]: "inv_register_map (case_register hp ep (Suc 0) 0) 0 (Con 0) = 
+lemma [simp]: "inv_register_map (case_register hp ep (Suc 0) 0) 0 None = 
     case_reg (4 * hp) (Suc (4 * ep)) 6 3 0"
   by (auto split: reg.splits)
 
 lemma [dest]: "unmap_mem' x = (r, y) \<Longrightarrow> x = 4 * y + register_offset r"
   by (induction x arbitrary: y rule: unmap_mem'.induct) (simp_all split: prod.splits)
 
-lemma [simp]: "unmap_mem (case_register (\<lambda>x. (Con 0, 0)) (\<lambda>x. (Con 0, 0)) (\<lambda>x. (Con 0, 0)) 
-  ((\<lambda>x. (Con 0, 0))(0 := (PC 0, 0), Suc 0 := (Reg Env, 0)))) = (\<lambda>x. 0)(7 := 1)"
+lemma [simp]: "unmap_mem (case_register (\<lambda>x. (None, 0)) (\<lambda>x. (None, 0)) (\<lambda>x. (None, 0)) 
+  ((\<lambda>x. (None, 0))(0 := (None, 0), Suc 0 := (Some Env, 0)))) = (\<lambda>x. 0)(7 := 1)"
 proof (rule, unfold unmap_mem_def)
   fix x
   obtain r p where R: "unmap_mem' x = (r, p)" by fastforce
   moreover hence "x = 4 * p + register_offset r" by auto
   ultimately have "pseudoreg_map ((case r of 
-        Stk \<Rightarrow> (\<lambda>x. (Con 0, 0))(0 := (PC 0, 0), Suc 0 := (Reg Env, 0)) 
-      | _ \<Rightarrow> (\<lambda>x. (Con 0, 0))) p) = ((\<lambda>x. 0)(3 := 0, 7 := 1)) x" 
+        Stk \<Rightarrow> (\<lambda>x. (None, 0))(0 := (None, 0), Suc 0 := (Some Env, 0)) 
+      | _ \<Rightarrow> (\<lambda>x. (None, 0))) p) = ((\<lambda>x. 0)(3 := 0, 7 := 1)) x" 
     by (induction r) (simp_all, presburger+)
   with R show "(case unmap_mem' x of (r, p) \<Rightarrow> 
     pseudoreg_map ((case r of 
-      Stk \<Rightarrow> (\<lambda>x. (Con 0, 0))(0 := (PC 0, 0), Suc 0 := (Reg Env, 0)) | _ \<Rightarrow> (\<lambda>x. (Con 0, 0))) p)) =
+      Stk \<Rightarrow> (\<lambda>x. (None, 0))(0 := (None, 0), Suc 0 := (Some Env, 0)) | _ \<Rightarrow> (\<lambda>x. (None, 0))) p)) =
         ((\<lambda>x. 0)(7 := 1)) x" by simp
 qed
 
